Implement transitions

src/TM.v
@@ -1,5 +1,6 @@
 Set Warnings "-stdlib-vector".
-From Coq Require Vectors.Vector.
+From Coq Require Import Lists.List Vectors.Vector Vectors.Fin.
+Import ListNotations.
 From klenee_complexity Require Import NEList.
 
 Section TuringMachines.
@@ -20,52 +21,129 @@ Section TuringMachines.
         work_tapes_indices : Vector.t nat work_tapes_num;
     }.
 
-    Definition Trace  := NEList Conf.
+    Definition get_input_symbol (c : Conf) : option Σ :=
+        nth_error (input c) (input_index c).
+
+    Record TransitionCond := {
+        input_symbol : Σ;
+        work_tapes_symbols : Vector.t Γ work_tapes_num;
+    }.
+
+    Inductive Move := Left | Right | Stay. 
+
+    Record TransitionAction := {
+        new_work_tapes_symbols : Vector.t Γ work_tapes_num;
+        input_move : Move;
+        work_tapes_moves : Vector.t Move work_tapes_num;
+    }.
+
+    Definition update_index (idx : nat) (move : Move) : nat :=
+        match move with
+        | Left => 
+            match idx with
+            | 0 => 0
+            | S n => n
+            end
+        | Right => S idx
+        | Stay => idx
+        end.
+
+    Definition update_tape (tape : list Γ) (idx : nat) (new_sym : Γ) : list Γ :=
+        (fix replace_nth (l : list Γ) (n : nat) (x : Γ) : list Γ :=
+            match l, n with
+            | [], _ => []
+            | h :: t, 0 => x :: t
+            | h :: t, S n' => h :: replace_nth t n' x
+            end) tape idx new_sym.
+    
+    Definition work_tapes_consistent
+        (c1 c2 : Conf) 
+        (cond : TransitionCond) 
+        (action : TransitionAction) : Prop :=
+            forall (i : nat) (H : i < work_tapes_num),
+                let fin_idx := of_nat_lt H in
+
+                let tape1 := Vector.nth (work_tapes c1) fin_idx in
+                let idx1 := Vector.nth (work_tapes_indices c1) fin_idx in
+                let exp_sym := Vector.nth (work_tapes_symbols cond) fin_idx in
+                let tape2 := Vector.nth (work_tapes c2) fin_idx in
+                let idx2 := Vector.nth (work_tapes_indices c2) fin_idx in
+                let new_sym := Vector.nth (new_work_tapes_symbols action) fin_idx in
+                let mv := Vector.nth (work_tapes_moves action) fin_idx in
+                
+                (nth_error tape1 idx1 = Some exp_sym) /\
+                (tape2 = update_tape tape1 idx1 new_sym) /\
+                (idx2 = update_index idx1 mv).
+    
+
+    Record P := {
+        t_cond : TransitionCond;
+        t_action: TransitionAction;
+    }.
 
     Class TM := {
         init : Q;
         final : Q -> bool;
 
-        transitions : Type;
-        do_transition : Conf -> Conf;
+        exist_transition : P -> Conf -> Conf -> Prop;
     }.
+
+    Definition DTransitions := Q * TransitionCond -> Q * TransitionAction.
 
     Record DTM := {
         d_init : Q;
         d_final : Q -> bool;
+
+        d_transitions : DTransitions;
     }.
 
-    Inductive Move := Left | Right | Stay. 
-
-    Definition DTransitions (n : nat) :=
-        Q * Σ * (Vector.t Γ n) -> 
-        Q * (Vector.t Γ n) * Move * (Vector.t Move n).
+    Definition exist_d_transition (d_transitions : DTransitions) (p : P) (c1 c2 : Conf) := 
+        let (cond, action) := p in
+        let (expected_new_state, expected_action) := d_transitions (state c1, cond) in
+        
+        (get_input_symbol c1 = Some (input_symbol cond)) /\
+        (expected_action = action) /\
+        (expected_new_state = state c2) /\
+        (input c2 = input c1) /\
+        (input_index c2 = update_index (input_index c1) (input_move action)) /\
+        (work_tapes_consistent c1 c2 cond action).
 
     Global Instance DTM_TM (dtm : DTM) : TM :=
     {|
         init := d_init dtm;
         final := d_final dtm;
 
-        transitions := DTransitions work_tapes_num;
-        do_transition := id; (*TODO*)
+        exist_transition := exist_d_transition (d_transitions dtm);
     |}.
+
+    Definition NTransitions := Q * TransitionCond -> list (Q * TransitionAction).
 
     Record NTM := {
         n_init : Q;
         n_final : Q -> bool;
+
+        n_transitions : NTransitions;
     }.
 
-    Definition NTransitions (n : nat) :=
-        Q * Σ * (Vector.t Γ n) -> 
-        list (Q * (Vector.t Γ n) * Move * (Vector.t Move n)).
+    Definition exist_n_transition (n_transitions : NTransitions) (p : P) (c1 c2 : Conf) := 
+        let (cond, action) := p in
+        let possible_transitions := n_transitions (state c1, cond) in
+        
+        (get_input_symbol c1 = Some (input_symbol cond)) /\
+        (exists (expected_state : Q) (expected_action : TransitionAction),
+            List.In (expected_state, expected_action) possible_transitions /\
+            expected_action = action /\
+            expected_state = state c2) /\
+        (input c2 = input c1) /\
+        (input_index c2 = update_index (input_index c1) (input_move action)) /\
+        (work_tapes_consistent c1 c2 cond action).
 
     Global Instance NTM_TM (ntm : NTM) : TM :=
     {|
         init := n_init ntm;
         final := n_final ntm;
 
-        transitions := NTransitions work_tapes_num;
-        do_transition := id; (*TODO*)
+        exist_transition := exist_n_transition (n_transitions ntm);
     |}.
 
     Inductive QType := Existential | Universal.
@@ -75,6 +153,7 @@ Section TuringMachines.
         a_final : Q -> bool;
 
         q_type : Q -> QType;
+        a_transitions : NTransitions;
     }.
 
     Global Instance ATM_TM (atm : ATM) : TM :=
@@ -82,20 +161,34 @@ Section TuringMachines.
         init := a_init atm;
         final := a_final atm;
 
-        transitions := NTransitions work_tapes_num;
-        do_transition := id; (*TODO*)
+        exist_transition := exist_n_transition (a_transitions atm);
     |}.
 End TuringMachines.
 
-Definition transition `{TMParams} (tm : TM) (conf1 conf2 : Conf) : Prop :=
-    do_transition conf1 = conf2.
+Definition transition `{TMParams} (tm : TM) (p : P) (conf1 conf2 : Conf) : Prop :=
+    exist_transition p conf1 conf2.
 
-Notation "conf1 ⊢ᶜ conf2" := (transition _ conf1 conf2) (at level 70).
+Notation "conf1 ○ p ⊢ᶜ conf2" := (transition _ p conf1 conf2) (at level 70).
 
-Definition ttransition `{TMParams} (tm : TM) (trace1 trace2 : Trace) : Prop :=
-    let head1 := head trace1 in
-    let head2 := head trace2 in
-        trace2 = cons head2 (trace1) /\
-        head1 ⊢ᶜ head2.
+Definition Trace `{TM} := 
+    { t : NEList Conf |
+        let confs := toList t in
+        (fix check_confs (cs : list Conf) (prev : option Conf) : Prop :=
+            match cs, prev with
+            | [], _ => True
+            | c :: rest, None => check_confs rest (Some c)
+            | c :: rest, Some prev_c =>
+                exists (p : P), prev_c ○ p ⊢ᶜ c /\
+                check_confs rest (Some c)
+            end) confs None }.
 
-Notation "trace1 ⊢ trace2" := (ttransition _ trace1 trace2) (at level 70).
+Definition ttransition `{TMParams} (tm : TM) (p : P) (trace1 trace2 : Trace) : Prop :=
+    match trace1, trace2 with
+    | exist _ t1 _, exist _ t2 _ =>
+        let head1 := head t1 in
+        let head2 := head t2 in
+            t2 = cons head2 (t1) /\
+            head1 ○ p ⊢ᶜ head2
+    end.
+
+Notation "trace1 ○ p ⊢ trace2" := (ttransition _ p trace1 trace2) (at level 70).
